PiLL/PiLL/Framework/Semantics/EnvStep.lean
@@ -57,7 +57,8 @@ inductive EnvStep : HyperEnv → Lbl → HyperEnv → Prop where
 
   | res
       {𝒢 𝒢' : HyperEnv} {Γ Γ' Δ Δ' : Env} {x y : FPName} {A B : Types} {l : Lbl}
-      {hFx : x ∉ (𝒢' |ₕ [Γ'‚ Δ']).names} {hFy : y ∉ (𝒢' |ₕ [Γ'‚ Δ']).names} :
+      {hFx : x ∉ (𝒢 |ₕ [Γ‚ Δ]).names} {hFy : y ∉ (𝒢 |ₕ [Γ‚ Δ]).names} :
+    --   {hFx : x ∉ (𝒢' |ₕ [Γ'‚ Δ']).names} {hFy : y ∉ (𝒢' |ₕ [Γ'‚ Δ']).names} :
       EnvStep (𝒢 |ₕ [x ∶ Aᗮ :: Γ] |ₕ [y ∶ A :: Δ]) (l) (𝒢' |ₕ [x ∶ Aᗮ :: Γ'] |ₕ [y ∶ A :: Δ']) →
       -------------------------------------------------------------------------------------
       EnvStep (𝒢 |ₕ [Γ‚ Δ]) l (𝒢' |ₕ [Γ'‚ Δ'])
@@ -146,46 +147,48 @@ inductive MEST : (𝒢 : HyperEnv) → Lbls → (𝒢' : HyperEnv) → Prop wher
 
 notation:50 𝒢 " -[" ls "]->>ₑ " 𝒢' => MEST 𝒢 ls 𝒢'
 
-@[simp] lemma EnvStep.names_subset {𝒢 𝒢' : HyperEnv} {l : Lbl} :
-  (𝒢 -[l]->ₑ 𝒢') → 𝒢'.names ⊆ 𝒢.names ∪ l.i := by
-  intro h
-  induction h
-  case tensor | parr =>
-    simp ; rw [Finset.insert_comm]
 
-  case par₁ | par₂ =>
-    grind [HyperEnv.names_merge]
 
-  case syn =>
-    grind [HyperEnv.names_merge, Lbl.i]
+-- @[simp] lemma EnvStep.names_subset {𝒢 𝒢' : HyperEnv} {l : Lbl} :
+--   (𝒢 -[l]->ₑ 𝒢') → 𝒢'.names ⊆ 𝒢.names ∪ l.i := by
+--   intro h
+--   induction h
+--   case tensor | parr =>
+--     simp ; rw [Finset.insert_comm]
 
-  case res 𝒢 𝒢' Γ Γ' Δ Δ' x y _ _  l hFx hFy  _ ih =>
-    simp_all only [HyperEnv.names_merge, HyperEnv.names_singleton, Env.names_merge,
-      Env.names_distributes, Lbl.i, Finset.mem_union]
-    intro n hn
+--   case par₁ | par₂ =>
+--     grind [HyperEnv.names_merge]
 
-    simp only [Finset.mem_union] at hn
+--   case syn =>
+--     grind [HyperEnv.names_merge, Lbl.i]
 
-    have hnx : n ≠ x := by rintro rfl ; exact hFx hn
-    have hny : n ≠ y := by rintro rfl ; exact hFy hn
+--   case res 𝒢 𝒢' Γ Γ' Δ Δ' x y _ _  l hFx hFy  _ ih =>
+--     simp_all only [HyperEnv.names_merge, HyperEnv.names_singleton, Env.names_merge,
+--       Env.names_distributes, Lbl.i, Finset.mem_union]
+--     intro n hn
 
-    have hinLHS : n ∈ 𝒢'.names ∪ ({x} ∪ Γ'.names) ∪ ({y} ∪ Δ'.names) := by
-      simp only [Finset.mem_union, Finset.mem_singleton]
-      rcases hn with h𝒢 | hΓ | hΔ <;> grind
+--     simp only [Finset.mem_union] at hn
 
-    have hPrev:= ih hinLHS
-    simp only [Finset.mem_union, Finset.mem_singleton] at ⊢ hPrev
-    rcases hPrev with ((h𝒢 | (hx | hΓ)) | (hy | hΔ)) | hM <;> grind
+--     have hnx : n ≠ x := by rintro rfl ; exact hFx hn
+--     have hny : n ≠ y := by rintro rfl ; exact hFy hn
 
-  case perm hP _ hP' ih =>
-    have heq := HyperEnv.names_eq_of_perm hP
-    have heq' := HyperEnv.names_eq_of_perm hP'
-    rw [← heq, ← heq']
-    exact ih
+--     have hinLHS : n ∈ 𝒢'.names ∪ ({x} ∪ Γ'.names) ∪ ({y} ∪ Δ'.names) := by
+--       simp only [Finset.mem_union, Finset.mem_singleton]
+--       rcases hn with h𝒢 | hΓ | hΔ <;> grind
 
-  all_goals simp
+--     have hPrev:= ih hinLHS
+--     simp only [Finset.mem_union, Finset.mem_singleton] at ⊢ hPrev
+--     rcases hPrev with ((h𝒢 | (hx | hΓ)) | (hy | hΔ)) | hM <;> grind
 
-lemma EnvStep.preserves_disjoint {𝒢 𝒢' ℋ : HyperEnv} {l : Lbl}
-  (hES : 𝒢 -[l]->ₑ 𝒢') (hD : 𝒢.disjoint ℋ) (hFl : Disjoint l.i ℋ.names) :
-  𝒢'.disjoint ℋ := by
-  exact Disjoint.mono_left (EnvStep.names_subset hES) (Finset.disjoint_union_left.mpr ⟨hD, hFl⟩)
+--   case perm hP _ hP' ih =>
+--     have heq := HyperEnv.names_eq_of_perm hP
+--     have heq' := HyperEnv.names_eq_of_perm hP'
+--     rw [← heq, ← heq']
+--     exact ih
+
+--   all_goals simp
+
+-- lemma EnvStep.preserves_disjoint {𝒢 𝒢' ℋ : HyperEnv} {l : Lbl}
+--   (hES : 𝒢 -[l]->ₑ 𝒢') (hD : 𝒢.disjoint ℋ) (hFl : Disjoint l.i ℋ.names) :
+--   𝒢'.disjoint ℋ := by
+--   exact Disjoint.mono_left (EnvStep.names_subset hES) (Finset.disjoint_union_left.mpr ⟨hD, hFl⟩)
